# Article for infinite product with [signature](../product_signature.html) 9:(0,-1,1,0,0,1,-1,0,0) 

!!graphs

$$ F(q) := \sum_{n=0}^\infty r(n)q^n := \frac{f(-q^2,-q^7)}{(q^3;q^3)_\infty} = \frac{(q^{2},q^{7}; q^{9})_\infty}{(q^{3},q^{6}; q^{9})_\infty} $$

## Power series expansion

!!power_series

## $q$-series representations

$ \displaystyle F(q) = \sum_{n=0}^\infty \frac{q^{3n(n+1)}(q;q)_{3n}(1-q^{3n+2})}{(q^3;q^3)_{n}(q^3;q^3)_{2n+1}}$

**Common name:** The second Bailey mod 9 identity


**[Bailey pair](../Bailey_pairs.html) proof:**
> PROOF HERE OR DELETE THIS LINE

**Combinatorial interpretations:**
- 1st interpretation here
- 2nd interpretation here

**Notes:**
- Due to Bailey (1943, p. 422, Eq. (1.7)).
- Slater (41, corrected).

## References
- Ref 1 here
- Ref 2 here
