# Article for infinite product with [signature](../product_signature.html) 4:(1, -2, 1, 0)

!!graphs

$$ F(q) :=\sum_{n=0}^\infty r(n)q^n := \frac{f(-q^2, -q^2)}{\psi(-q)} = \frac{(q^2;q^4)_\infty^2}{(q,q^3;q^4)_\infty} $$


## [Asymptotic formula](../asymptotics.html)

$ \displaystyle r(n) \sim FORMULA\;HERE $ as $ n\to\infty. $

## Power series expansion

!!power_series

## $q$-series representations

$ \displaystyle F(q) = \sum_{n=0}^\infty \frac{q^{n^2}(q;q^2)_n}{(q^4;q^4)_n} $

**[Bailey pair](../Bailey_pairs.html) proof:** PROOF HERE OR DELETE THIS LINE

**Combinatorial interpretations:**
- 1st interpretation here
- 2nd interpretation here
    
**Notes:**
- Special case $(a^2 = -c = q)$ of $q$-Gauss
- Slater (4) with $q\to -q$.


    
## References
- Ref 1 here
- Ref 2 here
